lib/CoqlibC.v
@@ -144,6 +144,8 @@ Notation top1 := (fun _ => True).
 Notation top2 := (fun _ _ => True).
 Notation top3 := (fun _ _ _ => True).
 Notation top4 := (fun _ _ _ _ => True).
+Notation top5 := (fun _ _ _ _ _ => True).
+Notation top6 := (fun _ _ _ _ _ _ => True).
 
 Notation " 'all1' p" := (forall x0, p x0) (at level 50, no associativity, only parsing).
 Notation " 'all2' p" := (forall x0 x1, p x0 x1) (at level 50, no associativity, only parsing).
